 
\documentclass{llncs}

\usepackage{listings}
\usepackage{amssymb}
\usepackage[margin=.9in]{geometry}
\usepackage{amsmath}
%\usepackage{amsthm}
\usepackage{mathpartir}
\usepackage{color,soul}

%\theoremstyle{definition}
%%\newtheorem{case1}{Case1}
\spnewtheorem{casethm}{Case}[theorem]{\itshape}{\rmfamily}
\spnewtheorem{subcase}{Subcase}{\itshape}{\rmfamily}
\numberwithin{subcase}{casethm}
\numberwithin{casethm}{theorem}
\numberwithin{casethm}{lemma}




\lstdefinestyle{custom_lang}{
  xleftmargin=\parindent,
  showstringspaces=false,
  basicstyle=\ttfamily,
  keywordstyle=\bfseries
}

\lstset{emph={%  
    val, def, type, new, z%
    },emphstyle={\bfseries \tt}%
}

\begin{document}
\hl{*Note highlighted text implies more work is needed.}

%---------------------- Preservation ----------------------%
\begin{theorem}[Preservation]
If $\Gamma; \Sigma \vdash e : T$, 
   	$\mu \; | \; e \; \rightarrow \mu' \; | \; e'$ where
	$\Sigma \vdash \mu \; \tt{\bf{wf}}$ then 
 	$\exists \Sigma'$ s.t. 
	$\Sigma'$ extends $\Sigma$, 
	$\Sigma' \vdash \mu' \; \tt{\bf{wf}}$, 
	$\Gamma; \Sigma' \vdash e' : T$.
\end{theorem}

\begin{proof}
By induction on the derivation of $\mu \; | \; e \; \rightarrow \mu' \; | \; e'$.
\begin{casethm}[\textsc{R-New}]
 \begin{mathpar}
\inferrule
  {\mu \vdash \overline{d_v} \leadsto \overline{d} \\
  	l \notin dom(\mu) \\
  	\mu' = \mu, l \mapsto \{\texttt{z} \Rightarrow \overline{d}\}}
  {\mu \; | \; \texttt{new} \; \{\texttt{z} \Rightarrow \overline{d_v}\} \; \rightarrow \mu' \; | \; l}
	\and
\inferrule
	{\Gamma, z : \{z \Rightarrow \overline{\sigma}\}; \Sigma 
	\vdash \overline{d_v} : \overline{\sigma} \\
	y \notin dom(\Gamma)}
	{\Gamma; \Sigma\vdash \texttt{new} \; \{z \Rightarrow \overline{d_v}\} : 
	\{z \Rightarrow \overline{\sigma}\}}
\end{mathpar}
Let $\Sigma' = \Sigma, (l:\{z \Rightarrow \overline{\sigma}\})$.
By Lemma \ref{lem:path_type_preservation}, we can show that 
$\Gamma; \Sigma' \vdash \{\texttt{z} \Rightarrow \overline{d}\} :
\{z \Rightarrow \overline{\sigma}\}$. Thus by \textsc{T-Loc} we get the result 
$\Gamma; \Sigma' \vdash l : \{z \Rightarrow \overline{\sigma}\}$.
\end{casethm}

\begin{casethm}[\textsc{R-Meth}]
\begin{mathpar}
\inferrule
  {\mu \vdash v_1 \leadsto l \\
  	\mu(l) = \{\texttt{z} \Rightarrow ...,m:T(x:S)=e,...\}}
  {\mu \; | \; v_1.m_U(v_2) \;\rightarrow \mu \; | \; [v_1/z,v_2 \unlhd S/x]e \unlhd U}
	\and
\inferrule
  {\Gamma; \Sigma \vdash v_1 \ni \texttt{def} \; m:S' \rightarrow T' \\
  	\Gamma; \Sigma \vdash v_1 : T_1 \\
  	\Gamma; \Sigma \vdash v_2 : S' \\
  	\Gamma; \Sigma \vdash T' <: U}
  {	\Gamma; \Sigma \vdash v_1.m_U(v_2) : U}
\end{mathpar}
By Lemma \ref{lem:path_type_preservation} we know that 
$\Gamma; \Sigma \vdash l : T_1$. From Lemma \ref{lem:subtype:decl} 
we can show that $\Gamma; \Sigma \vdash [v_1/z](\texttt{def} \; m:S \rightarrow T) <:
\texttt{def} \; m:S' \rightarrow T'$ which implies 
$\Gamma; \Sigma \vdash [v_1/z] T <: T'$. Since 
$\Gamma; \Sigma \vdash e : T$, by Lemma \ref{lem:subst} 
we get $\Gamma; \Sigma \vdash [v_1/z,v_2 \unlhd S/x]e : [v_1/z,v_2 \unlhd S/x]T$.
Since $T$ is well-formed in the absence of $x$, 
$[v_1/z,v_2 \unlhd S/x]T = [v_1/z]T$. Thus we get 
$\Gamma; \Sigma \vdash [v_1/z,v_2 \unlhd S/x]e : [v_1/z]T$, and by 
\textsc{T-Sub} we have 
$\Gamma; \Sigma \vdash [v_1/z,v_2 \unlhd S/x]e : T'$ and subsequently 
$\Gamma; \Sigma \vdash [v_1/z,v_2 \unlhd S/x]e : U$. 
Now, let $\Sigma' = \Sigma$, and by \textsc{T-Type} 
we have $\Gamma; \Sigma' \vdash [v_1/z,v_2 \unlhd S/x]e \unlhd U : U$

\end{casethm}
\begin{casethm}[\textsc{R-Context}]
\begin{mathpar}
\inferrule
  {	\mu \; | \; e \; \rightarrow \; \mu' \; | \; e'}
  {\mu \; | \; E[e] \; \rightarrow \mu' \; | \; E[e']}
\end{mathpar}
By case analysis on $E[e]$.
\begin{subcase}[$\mu \; | \; e.m_U(e_S) \; \rightarrow \mu' \; | \; e'.m_U(e_S)$]
\begin{mathpar}
\inferrule
  {\Gamma; \Sigma \vdash e \ni \texttt{def} \; m:S' \rightarrow T' \\
  	\Gamma; \Sigma \vdash e : T \\
  	\Gamma; \Sigma \vdash e_S : S' \\
  	\Gamma; \Sigma \vdash T' <: U}
  {	\Gamma; \Sigma \vdash e.m_U(e_S) : U}
\end{mathpar}
By our induction hypothesis we assume 
$\Gamma; \Sigma' \vdash e' : T$. We now need to investigate 
method membership for $e'$. Since $e$ reduces to $e'$, we can be
sure that $e$ is not a path. By inversion on 
$\Gamma; \Sigma \vdash e \ni \texttt{def} \; m:S' \rightarrow T'$ it
follows that since $e$ is not a path, $z \notin \texttt{def} \; m:S' \rightarrow T'$. 
Thus $\Gamma; \Sigma' \vdash e' \ni \texttt{def} \; m:S' \rightarrow T'$, since 
no substitution is required. By simple weakening of the store type (\hl{TODO?})
the following hold.
\begin{mathpar}
\inferrule
  {\Gamma; \Sigma' \vdash e_S : S' \\
  	\Gamma; \Sigma' \vdash T' <: U}
  {}
\end{mathpar}
By \textsc{T-Meth} we have $\Gamma; \Sigma' \vdash e.m_U(e_S) : U$
\end{subcase}

\begin{subcase}[$\mu \; | \; p.m_U(e) \; \rightarrow \mu' \; | \; p.m_U(e')$]
\begin{mathpar}
\inferrule
  {\Gamma; \Sigma \vdash p \ni \texttt{def} \; m:S \rightarrow T \\
  	\Gamma; \Sigma \vdash p : T_p \\
  	\Gamma; \Sigma \vdash e : S \\
  	\Gamma; \Sigma \vdash T <: U}
  {	\Gamma; \Sigma \vdash p.m_U(e) : U}
\end{mathpar}
By our induction hypothesis we assume 
$\exists \Sigma' : \Gamma; \Sigma \vdash e : S$, where 
$\Sigma'$ extends $\Sigma$. By simple weakening of the store type (\hl{TODO?})
we get
\begin{mathpar}
\inferrule
  {\Gamma; \Sigma' \vdash p \ni \texttt{def} \; m:S \rightarrow T \\
  	\Gamma; \Sigma' \vdash p : T_p \\
  	\Gamma; \Sigma' \vdash T <: U}
  {}
\end{mathpar}
Thus by 
\textsc{T-Meth}, $\Gamma; \Sigma' \vdash p.m_U(e') : U$
\end{subcase}

\begin{subcase}[$\mu \; | \; e.f \; \rightarrow \mu' \; | \; e'.f$]
\begin{mathpar}
\inferrule
  {	\Gamma; \Sigma \vdash e : S \\
  	\Gamma; \Sigma \vdash e \ni \texttt{val} \; f:T}
  {	\Gamma; \Sigma \vdash e.f : T}
\end{mathpar}
By our induction hypothesis we assume $\Gamma; \Sigma \vdash e' : S$. 
Since $e$ reduces to $e'$ it follows that $e$ is not a path. By inversion 
on the derivation of $\Gamma; \Sigma \vdash e \ni \texttt{val} \; f:T$, 
$z \notin \texttt{val} \; f:T$, and it follows that 
$\Gamma; \Sigma' \vdash e' \ni \texttt{val} \; f:T$. Now, by \textsc{T-Field} 
we have $\Gamma; \Sigma' \vdash e'.f : S$
\end{subcase}

\begin{subcase}[$\mu \; | \; e \unlhd T \; \rightarrow \mu' \; | \; e' \unlhd T$]
\begin{mathpar}
\inferrule
  {	\Gamma; \Sigma \vdash e : T}
  {	\Gamma; \Sigma \vdash e \unlhd T : T}
\end{mathpar}
By our induction hypothesis we assume $\Gamma; \Sigma' \vdash e' : T$. 
Now by the simple application of \textsc{T-Type} we have 
$\Gamma; \Sigma' \vdash e' \unlhd : T$
\end{subcase}

\end{casethm}
\end{proof}
\qed

%---------------------- Progress ----------------------%
\subsection{Progress}
\begin{theorem}[Progress]
If $\Gamma \vdash e : T$, then either
\begin{enumerate}
\item e is a value, or
\item $\forall \mu$ s.t.
		   $\Gamma \vdash \mu$,
         $\exists e'$ and $\mu'$ s.t. 
         $\mu \; | \; e \; \rightarrow \mu' \; | \; e'$
\end{enumerate}
\end{theorem}
\qed 






\bibliographystyle{plain}
\bibliography{bib}

\end{document}