\documentclass{article}
\usepackage{mathpartir}
\usepackage{cite}
\usepackage{graphicx}
\usepackage{amsmath,fullpage,amssymb}

\newcommand{\typeexample}[2]{$#1$\\$#2$}
\newcommand{\st}{\ensuremath{\hspace{-1px}<:\hspace{-1px}}}
\newcommand{\alphahat}{\hat{\alpha}}
\newcommand{\betahat}{\hat{\beta}}

\newcommand{\botbound}{\sigma_{l}}
\newcommand{\topbound}{\sigma_{u}}

\newcommand{\marker}[1]{{\scriptscriptstyle {\blacktriangleright #1}}}

\newcommand{\lub}{\ensuremath{\vee}}
\newcommand{\glb}{\ensuremath{\wedge}}

\newcommand{\siglub}{\underbar{\lub}}
\newcommand{\sigglb}{\overset{\sigma}{\glb}}


\newcommand{\instr}{\overset{<}{=:}}
\newcommand{\instl}{\overset{<}{:=}}

\newcommand{\bndr}{\instr}
\newcommand{\bndl}{\instl}

\newcommand{\sigbndl}{:<\hspace{-5px}<}
\newcommand{\sigbndr}{<\hspace{-5px}<:}

\newcommand{\siginstr}{\overset{\overline{<}}{=:}}
\newcommand{\siginstl}{\overset{\overline{<}}{:=}}

\newcommand{\ctxtsep}{;}
\newcommand{\ctxbsep}{;}

\newcommand{\tst}{{\scriptstyle{<:}}}
\newcommand{\bound}[3]{#1 \tst #2 \tst #3}

\newcommand{\analyzes}{\ensuremath{\Leftarrow}}
\newcommand{\synth}{\ensuremath{\Rightarrow}}

\newcommand{\fnSynth}{\synth\hspace{-5px}\synth}

\newcommand{\pronounce}[2]{{\makebox[\linewidth][l]{\framebox{#1} \parbox{\textwidth}{#2}}}}

\newcounter{labctr}
\newcommand{\la}[1]{\refstepcounter{labctr}\label{#1}\arabic{labctr})\>}
\newcommand{\resla}{\setcounter{labctr}{0}}

\renewcommand{\and}{\text{ and }}
\newcommand{\ctxmapto}{\longmapsto}

\newcommand{\pair}[2]{\left<#1,#2\right>}
\newcommand{\arrow}[2]{#1 \rightarrow #2}

\newcommand{\typeset}{\Xi}
\begin{document}

\section{Instantiation Completeness}

Given that $\Gamma \longmapsto \Omega$, $A=[\Gamma]A$, and $\Gamma = \Gamma_1,\bound{\sigma_l}{\alphahat}{\sigma_u},\Gamma_2$\\
if $[\Omega]\Gamma\vdash [\Omega]\alphahat \leq [\Omega]A$, then there are some $\Delta,\Omega'$ such that $\Gamma \vdash \alphahat \instl A \dashv \Delta$, $\Delta \longmapsto \Omega'$, and $\Omega \longrightarrow \Omega'$.\\
if $[\Omega]\Gamma\vdash [\Omega]A \leq [\Omega]\alphahat$, then there are some $\Delta,\Omega'$ such that $\Gamma \vdash A \instr \alphahat \dashv \Delta$, $\Delta \longmapsto \Omega'$, and $\Omega \longrightarrow \Omega'$.

We proceed by structural induction on A.
\begin{tabbing}
Case \=$A = 1$\\
\la{initial1}$[\Omega]\Gamma \vdash [\Omega]\alphahat \leq [\Omega]A$ \` Given.\\
\la{initial2}$[\Omega]\Gamma \vdash [\Omega]\alphahat \leq 1$ \` $A = 1$ as given.\\
\la{initiala}$[\Omega]\alphahat = 1$ \` Inversion of $\st$Unit and predicative $\Omega$.\\
\la{initial3}$[\Omega]\Gamma \vdash [\Omega]\alphahat \leq 1$ \` By definition of $\Omega$\\
\>Want to find $\Delta$ such that $\Gamma \vdash \alphahat \instl 1 \dashv \Delta$ by applying rule InstLAbs.\\
\la{gammadecomp} $\Gamma = \Gamma_1,\bound{\sigma_l}{\alphahat}{\sigma_t},\Gamma_2$\` As $\Gamma \ctxmapto\Omega$ and $\Omega$ contains $\alphahat$\\
\la{bnd}$\Gamma_1\vdash \sigma_l \sigbndl 1 \dashv \Theta$ \` By lemma 10 on $\Gamma \ctxmapto \Omega$ and \ref{initiala}\\
\>This provides us with the first clause in InstLAbs.\\
\>We now need to show that some new bound exists with the given constraint\\
\la{bnd2}$\Theta \ctxmapto \Omega$ \` lemma 10 on $\Gamma \mapsto \Omega$\\
\la{lub}$\Theta\vdash \sigma_u \lub 1 = \pair{\rho}{1} \dashv \Theta$\\
\>\hspace{1em}\=Case \=$\sigma_u = \pair{\rho}{\tau_u}$\\
\>\>\la{abnd}$\Gamma\vdash 1 \sigbndr \pair{\rho}{\tau_u} \dashv\_$ \` lemma 10 on $\Gamma \ctxmapto \Omega$ and \ref{initiala}\\
\>\>\la{abndsub}$\Gamma\vdash 1 \sigbndr \pair{\emptyset}{\tau_u} \dashv\_$ \` lemma 14 on \ref{abnd}\\
\>\>\la{rep}$\Theta''\vdash 1\st\tau_u \dashv\Theta'$ \` Inversion of rule BndLType on \ref{abndsub}\\
\>\>\>$\tau_u = 1$ \` As $\tau_u$ a monotype, the only rule that can apply is $\st$Unit.\\
\>\>\la{cp5}$\Theta \vdash 1 \veebar 1 =1  \dashv \Theta$ \` By $\veebar$L on \ref{rep}\\
\>\>\la{c1}$\Theta \vdash \pair{\rho}{1} \lub 1 = \pair{\rho}{1}\dashv\Theta$ \` By $\lub\tau$ on \ref{cp5}\\
\>\>Case \=$\sigma_u = \pair{\rho}{\top}$\\
\>\>\la{c2}$\Theta[\alphahat \st \sigma_u] \vdash \pair{\rho}{\top} \lub 1 = \pair{\rho}{1} \dashv \Theta$ \` By $\lub\top$.\\
\>\>Case \=$\sigma_u = \pair{\rho}{\bot}$\\
\>\>\la{ctra1}$\Theta \vdash [\Omega]\alphahat \sigbndr \pair{\rho}{\bot} \dashv\Theta'$\\
\>\>\>$\Theta''\vdash [\Omega]\alphahat \sigbndr \pair{\emptyset}{\bot} \dashv \Theta'$ \` lemma 17 on \ref{ctra1}\\
\>\>\la{ctra}Contradiction, no rule exists\\
\la{app}$\Gamma[\bound{\sigma_l}{\alphahat}{\sigma_u}]\vdash \alphahat \instl 1 \dashv \Theta,\bound{\sigma_l}{\alphahat}{\pair{\rho}{1}},\Gamma_2$ \` By InstLAbs on \ref{bnd}, \ref{lub}\\
\>Choose $\Delta = \Theta,\bound{\sigma_l}{\alphahat}{\pair{\rho}{1}},\Gamma_2$\\
\>Choose $\Omega' = \Omega$\\
\> $\Omega \longrightarrow \Omega'$ \` By Dunfield lemma 20 (reflexivity).\\
\> We want to show that $\Delta \ctxmapto \Omega$. This will satisfy the completeness theorem in this case.\\
\> $\Delta = \Theta,\bound{\sigma_l}{\alphahat}{\pair{\rho}{1}},\Gamma_2$ 	\` By defn. of $\Delta$\\
\> $\Omega = \Omega_u,\alphahat = 1,\Omega_l$							\` By defn. of $\Omega$ and $[\Omega]\alphahat=1$\\
\> We proceed by showing the requisite piecewise properties, then reconstructing the relationship\\
\> between $\Delta$ and $\Omega$\\
%\la{l101} $\Gamma_2 \ctxmapto \Omega_l$ 										\` lemma 10 on $\Gamma \ctxmapto\Omega$\\
\la{l103} $\Gamma_1 \vdash 1 \sigbndr \sigma_u \dashv \Theta_u''$ 				\` \emph{ibid}\\
 WTS: $\Theta \vdash 1 \sigbndr \pair{\rho}{1} \dashv \Theta_u''$\\
\la{unit} $\Theta_u'' \vdash 1 \st 1 \dashv \Theta_u''$ 						\` by $\st$Unit\\
\la{inifn} $\Theta \vdash 1 \sigbndr \pair{\rho}{\tau_u} \dashv \Theta_k$ \` By lemma 10 on $\Gamma \ctxmapto\Omega$\\
\la{fn} $\Theta \vdash 1 \sigbndr \pair{\rho}{\top} \dashv\Theta_u''$				\` By lemma 26 on \ref{bnd}, \ref{unit}, and on \ref{inifn}\\
\la{finally} $\Theta_u \vdash 1 \sigbndr \pair{\rho}{1} \dashv \Theta_u''$ 			\` By lemma 12 on \ref{unit} and \ref{fn}\\
\la{tighter} $\Gamma \hookrightarrow \Delta$ \` By tightening lemma on \ref{app}\\
\> $\Delta \mapsto \Omega$ \` By lemma 11 on \ref{tighter}, \ref{finally}, \ref{bnd}, and $\Gamma \mapsto \Omega$\\
Case \=$A = X$\resla\\
\la{basicC} $[\Omega]\Gamma \vdash [\Omega]\alphahat \leq [\Omega]A$ \` Given.\\
\la{step1C} $[\Omega]\Gamma \vdash [\Omega]\alphahat \leq X$ \` As $A = X$ on \ref{basicC}.\\
\la{inverC} $[\Omega]\alphahat = Y$ \` As $\tau$ atomic and by construction of $X$ and $Y$ on \ref{step1C}\\ 
\la{inverCi} $[\Omega]\Gamma \vdash Y \leq X$ \` By substitution in \ref{step1C} with \ref{inverC}\\ 
\la{innerSys} $ Y < X$ \` By inversion of $\leq$Gen on \ref{inverCi}\\ 
\la{decomp} $\Gamma = \Gamma',\bound{\sigma_l}{\alphahat}{\sigma_t},\Gamma''$ \` As $\alphahat$ is in $\Omega$ and $\Gamma \mapsto \Omega$\\
\la{clause05} $\Gamma' \vdash \sigma_l \sigbndl Y \dashv \Theta$ \` By lemma 4 on \ref{decomp} and \ref{inverC}.\\
\la{stup} $\Theta \vdash Y \st X \dashv \Theta$ \` By $\st$Gen on \ref{innerSys}\\
\la{clause1} $\Gamma' \vdash \sigma_l \sigbndl X \dashv \Theta$ \` By lemma 52 on \ref{stup} and \ref{clause05}\\
\la{lubref1}$\Theta\vdash \sigma_u \lub X = \pair{\rho}{Z} \dashv \Theta$ \` For some type $Z$\\
\la{lubref2}$\Theta\vdash X \st Z \dashv \Theta$\\
\>We prove \ref{lubref1} and \ref{lubref2} by case analysis on $\sigma_u$\\
\>Case $\sigma_u = \pair{\rho}{\tau_u}$\\
\>\>\la{abnd2}$\Gamma\vdash [\Omega]\alphahat \sigbndr \pair{\rho}{\tau_u} \dashv\Theta'$ \` lemma 10 on $\Gamma \ctxmapto \Omega$\\
\>\>\la{bnder2}$\Theta''\vdash[\Omega]\alphahat\st\tau_u \dashv\Theta'$ \` Lemma 7 on \ref{abnd2}\\
\>\>\la{repi}$\Theta''\vdash Y \st \tau_u \dashv\Theta'$ \` As $[\Omega]\alphahat = Y$\\
\>\>\la{inxi} $\tau_u = W$ \` By inversion of $\st$Gen on \ref{repi}\\
\>\>\la{bndi} $\Theta \vdash \pair{\rho}{\tau_u} \lub X = \pair{\rho}{Z} \dashv \Theta$ \` Inversion of $\lub$\\
\>\>\la{subs} $\Theta \vdash X \st Z \dashv \Theta$ \` By def. of upper bounding\\
\>Case $\sigma_u = \pair{\rho}{\top}$\\
\>\>\la{duh2} $\Theta \vdash \pair{\rho}{\top} \lub X = \pair{\rho}{X} \dashv \Theta$ \` By lemma 16\\
\>\>\la{subs2} $\Theta \vdash X \st X \dashv \Theta$ \` Reflexivity\\
\>Case $\sigma_u = \pair{\rho}{\bot}$\\
\>\>\la{abnd3c}$\Gamma\vdash [\Omega]\alphahat \sigbndr \pair{\rho}{\bot} \dashv\Theta'$ \` lemma 10 on $\Gamma \ctxmapto \Omega$\\
\>\>Contradiction, no type is subtype of $\bot$.\\
\>$\Gamma[\bound{\sigma_l}{\alphahat}{\sigma_u}]\vdash \alphahat \instl X \dashv \Theta,\bound{\sigma_l}{\alphahat}{\pair{\rho}{Z}},\Gamma_2$ \` By InstLAbs on \ref{clause1}, \ref{lubref1}\\
\>Choose $\Delta = \Theta,\bound{\sigma_l}{\alphahat}{\pair{\rho}{Z}},\Gamma_2$\\
\>Choose $\Omega' = \Omega$\\
\>$\Omega \longrightarrow \Omega'$ \` Dunfield, reflexivity\\
\>WTS: $\Gamma \mapsto \Delta$\\
\>Again, lemma 11 (rev.) is suggeseted here.\\
Case \=$A = \betahat$\resla\\
\>$\alphahat \neq \betahat$ 											\` $\alphahat \not\in FV(A)$\\
\la{st} $[\Omega]\Gamma \vdash [\Omega]\alphahat \leq [\Omega]\betahat$ 		\` $A = \betahat$\\
\la{t1} $[\Omega]\alphahat = \tau_1$ 										\` $\Omega$ predicative\\
\la{t2} $[\Omega]\betahat = \tau_2$ 											\` $\Omega$ predicative\\
\la{abs} $[\Omega]\Gamma \vdash \tau_1 \leq \tau_2$ 									\` Substituting \ref{t1} and \ref{t2} into \ref{st}\\
\> We want to eventually apply one of InstLReach or InstLVar depending on the order of the existential variables \\
\> in the context.\\
\> Let $\Omega' = \Omega$. We do not have to modify $\Omega$, as we add no new variables\\
\> $\Omega' \longrightarrow \Omega$ 									\` Dunfield lemma 20, reflexivity.\\
\> Case \=on $\alphahat$ left or right of $\betahat$\\
\>\>Case \=$\Gamma = (\Gamma_0,\alphahat,\Gamma_1,\bound{\sigma_l}{\betahat}{\sigma_t},\Gamma_2)$\\
\>\>In this case, $\betahat$ is below $\alphahat$ in the context, so we have to modify $\betahat$'s bounds to \\
\>\>maintain the ordering constraint.\\
\>\>\la{b1}$\Gamma_0,\alphahat,\Gamma_1 \vdash \tau_2 \sigbndr \sigma_t$		\` lemma 10 on $\Gamma \mapsto \Omega$\\
\>\>\la{b2}$\Gamma_0,\alphahat,\Gamma_1 \vdash \tau_1 \sigbndr \sigma_t$		\` lemma 8 on \ref{abs}\\
\>\>We have established that $\sigma_t$ bounds both result types from above. We now use this to bound $\alphahat$.\\
\>\>\la{ir}$\Gamma_0,\alphahat,\Gamma_1 \vdash \alphahat \sigbndr \sigma_t \dashv \Theta$	\` lemma 1 on \ref{b2}\\
\>\>\>$\Gamma_0,\alphahat,\Gamma_1,\betahat,\Gamma_2 \vdash \alphahat \instl \betahat \dashv \Theta,\bound{\pair{\{\alphahat,r\}}{c}}{\betahat}{\sigma_t},\Gamma_2$	\` InstLReach on \ref{ir}\\
\>\>We have now shown that InstLReach holds. We now need to show that the original solution still works.\\
\>\>\>$\Omega' = \Omega, \Delta = \Theta;\bound{\pair{\{\alphahat,r\}}{c}}{\betahat}{\sigma_t};\Gamma_2$\\
\>\>\>WTS: $\Theta,\bound{\pair{\{\alphahat,r\}}{c}}{\betahat}{\sigma_t},\Gamma_2 \ctxmapto \Omega_1,\betahat=\tau_2,\Omega_2$\\
\>\>We reconstruct the context using the context bound operators, satisfying the construction rule for the context.\\
\>\>\la{rel}$\Theta,\bound{\sigma_l}{\betahat}{\sigma_t},\Gamma_2 \ctxmapto \Omega_1,\betahat = \tau_2,\Omega_2$ \` By lemma 1 on \ref{b2}\\
\>\>\la{tot10} $\Gamma_2 \ctxmapto \Omega_2$ 										\` lemma 10 on \ref{rel}\\
\>\>\la{l1021} $\Theta \vdash \sigma_l \sigbndl \tau_2 \dashv \Theta'$ 			\` \emph{ibid}\\
\>\>\> $\Theta \vdash \tau_2 \sigbndr \sigma_t \dashv \Theta''$ 		\` \emph{ibid}\\
\>\>\> $\Theta''\ctxmapto\Omega$ 											\` \emph{ibid}\\
\>\>\la{thp} $\Theta'\ctxmapto\Omega$ 											\` \emph{ibid}\\
\>\>\> WTS: $\Theta \vdash \pair{\{\alphahat,r\}}{c} \sigbndl \tau_2 \vdash \Theta_f$ and $\Theta_f \ctxmapto \Omega$\\
\>\>\la{ihp} $[\Omega]\Theta\vdash [\Omega]\alphahat \leq \tau_2$ 			\` By lemma 18 on \ref{abs}, \ref{thp}, and $\Gamma \ctxmapto \Omega$ \\
\>\>\la{instlb} $\Theta \vdash \alphahat \instl \tau_2 \dashv \Theta_1$ 			\` By IH on \ref{ihp}.\\
\>\>\la{th1mt} $\Theta_1 \ctxmapto \Omega$												\` \emph{ibid}\\
\>\>\la{finth} $\Theta_1 \vdash \pair{\{r\}}{c} \sigbndl \tau_2 \dashv \Theta_f$ \` By lemma 21 on \ref{th1mt}, \ref{l1021}, \ref{ir} and lemma 22 on \ref{instlb}\\
\>\>\la{done} $\Theta \vdash \pair{\{\alphahat,r\}}{c} \sigbndl \tau_2 \vdash \Theta_f$		\` By BndLExt on \ref{finth} and \ref{instlb}\\
\>\>\> $\Theta,\bound{\pair{\{\alphahat,r\}}{c}}{\betahat}{\sigma_2},\Gamma_2 \ctxmapto \Omega_1,\betahat=\tau_2,\Omega_2$ \` By lemma 11 on \ref{done} and \ref{tot10}\\
\>\>Case \=$\Gamma = (\Gamma_0;\betahat;\Gamma_1;\bound{\sigma_l}{\alphahat}{\sigma_t};\Gamma_2)$\\
\>\>This is the converse to the above, where we use the similar InstLVar to modify $\alphahat$ instead of $\betahat$\\
\>\>\la{2b1}$\Gamma_0,\betahat,\Gamma_1 \vdash \sigma_l \sigbndl \tau_1$		\` lemma 10 on $\Gamma \mapsto \Omega$\\
\>\>\la{2b3}$\Gamma_0,\betahat,\Gamma_1 \vdash \sigma_l \sigbndl \tau_2$		\` lemma 23 on \ref{2b1}\\
\>\>\la{2ir}$\Gamma_0,\betahat,\Gamma_1 \vdash \sigma_l \sigbndl \betahat \dashv \Theta$	\` lemma 2 on \ref{2b3}\\
\>\>\la{2basis}$\Gamma_0,\betahat,\Gamma_1,\alphahat,\Gamma_2 \vdash \sigma_l \sigbndl \betahat \dashv \Theta,\bound{\sigma_l}{\alphahat}{\pair{\{r\}}{c}},\Gamma_2$	\` lemma 24 on \ref{2ir}\\
\>\>\>$\Gamma_0,\alphahat,\Gamma_1,\betahat,\Gamma_2 \vdash \alphahat \instl \betahat \dashv \Theta,\bound{\sigma_l}{\alphahat}{\pair{\{\betahat,r\}}{c}},\Gamma_2$	\` InstLVar on \ref{2basis}\\
\>\>\>$\Delta = \Theta,\bound{\sigma_l}{\alphahat}{\pair{\{\betahat,r\}}{c}},\Gamma_2$\\
\>\>\>WTS $\Delta \ctxmapto \Omega$\\
\>\>\la{omdef} $\Theta,\bound{\sigma_l}{\alphahat}{\pair{\{r\}}{c}},\Gamma_2 \ctxmapto \Omega_1,\alphahat=\tau_1,\Omega_2$ \` lemma 2 on \ref{2b3}\\
\>\>\> $\Theta \vdash \sigma_l \sigbndl \tau_2 \dashv \Theta'$  										\` lemma 10 on \ref{omdef}\\
\>\>\la{thm} $\Theta \vdash \tau_2 \sigbndr \sigma_t \dashv \Theta''$ 		\` \emph{ibid}\\
\>\>\la{thpm} $\Theta''\ctxmapto\Omega$ 											\` \emph{ibid}\\
\>\>\> $\Theta'\ctxmapto\Omega$ 											\` \emph{ibid}\\
\>\>\>Again, remains to finalize this.\\
Case $A = \arrow{A_1}{A_2}$\resla\\
\>Our main objective here is to end up applying InstLArrow. This rule is quite large, \\
\>and requires several judgements and contexts. Note that we use $\Theta_i$ consistently\\
\>between the rule and the proof.\\
\>$[\Omega]\Gamma \vdash [\Omega]\alphahat \leq [\Omega](\arrow{A_1}{A_2})$\` Given.\\
\>$[\Omega]\Gamma \vdash [\Omega]\alphahat \leq \arrow{([\Omega]A_1)}{([\Omega]A_2)}$\` By definition of context application\\
\>Since we have an arrow as the supertype, only $\leq\forall$L or $\st\rightarrow$ could have been used, and the subtype \\
\>$[\Omega]\alphahat$ must be either a quantifier or an arrow. But $\Omega$ is predicative, so $[\Omega]\alphahat$ cannot be a quantifier.\\
\>Therefore, it is an arrow: $[\Omega]\alphahat = \arrow{\tau_1}{\tau_2}$ and $\st\rightarrow$ concluded the derivation.\\
\la{declst1}$[\Omega]\Gamma \vdash \tau_1 \leq [\Omega]A_1$\` Inversion of $\leq\rightarrow$\\
\la{declst2}$[\Omega]\Gamma \vdash [\Omega]A_2 \leq \tau_2$\` \emph{ibid}.\\
\> Choose $\Omega' = \Omega[\alphahat_2 = \tau_2,\alphahat_1 = \tau_1,\alphahat=\arrow{\alphahat_1}{\alphahat_2}]$.\\
\> We choose these variables to satiate the rule InstLArrow.\\
\> $\Omega \longrightarrow \Omega'$ \` Dunfield, completeness of instantiation under arrow\\
\> Let $\Gamma' = \Gamma_1,\alphahat_2,\alphahat_1,\bound{\sigma_l}{\alphahat}{\sigma_t},\Gamma_2$\\
\> $\Gamma' \ctxmapto \Omega'$ \` By repeated application of lemma 27\\
\> WTS (premise 1): $\Gamma' \vdash \sigma_l \sigbndl \arrow{\alphahat_1}{\alphahat_2} \dashv \Theta_1$ \` For some $\Theta_1$\\
\la{taubnd} $\Gamma' \vdash \sigma_l \sigbndl \arrow{\tau_1}{\tau_2} \dashv \Theta$\\
\la{apbb} $\Gamma' \vdash \sigma_l \sigbndl \arrow{\alphahat_1}{\alphahat_2}\dashv\Theta_1$\` By lemma 28 on \ref{taubnd} and $\Gamma' \mapsto \Omega'$ and for some $\Theta_1$\\
\la{ctr1} $\Gamma' \hookrightarrow \Theta_1$ \` By lemma 30 on \ref{apbb}\\
\la{th1map} $\Theta_1 \ctxmapto \Omega'$ \`\emph{ibid}\\
\> WTS (premise 2): $\Theta_1 \vdash \arrow{\alphahat_1}{\alphahat_2} \sigbndr \sigma_t \dashv \Theta_2$ \` For some $\Theta_2$\\
\la{taubnd2} $\Theta_1 \vdash \arrow{\tau_1}{\tau_2} \sigbndr \sigma_t \dashv \Theta$ \` For some $\Theta$, by \ref{th1map}\\
\la{taubnd3} $\Theta_1 \vdash \arrow{\alphahat_1}{\alphahat_2} \sigbndr \sigma_t \dashv \Theta_2$ \` By lemma 29 on \ref{taubnd2} and \ref{th1map}\\
\la{th2map} $\Theta_2 \ctxmapto \Omega'$ \` \emph{ibid}\\
\la{ctr2} $\Theta_1 \hookrightarrow \Theta_2$ \` By lemma 31 on \ref{taubnd3}\\
\>$\sigma_l = \pair{\rho_l}{c_l}$\\
\la{glb} $\Theta_2\vdash\sigma_l \glb (\arrow{\alphahat_1}{\alphahat_2}) = \pair{\rho_l}{\arrow{\alphahat_1}{\alphahat_2}} \dashv \Theta_3$ \` By following case analysis\\
\>Case \=$\sigma_l = \pair{\rho}{\tau}$ \\
\>\la{tbndar}$\Gamma' \vdash \sigma_l \sigbndr \arrow{\tau_1}{\tau_2} \dashv \Theta$ \` As $[\Omega]\alphahat = \arrow{\tau_1}{\tau_2}$ and $\Gamma \ctxmapto \Omega$, for some $\Theta$\\
\>\>$\Theta' \vdash \tau \st \arrow{\tau_1}{\tau_2} \dashv\Theta$ \` By lemma 7 on \ref{tbndar} and \ref{th1map}, for some $\Theta'$\\
\>\>$\tau = \arrow{\tau_1'}{\tau_2'}$ \` Only $\st\rightarrow$ could have been used, as $\tau$ monotype. Thus, $\tau$ is an arrow.\\
\>\la{ast}$\Theta'_1 \vdash \arrow{\tau'_1}{\tau'_2} \st \arrow{\alphahat_1}{\alphahat_2} \dashv \Theta_1$ \` By lemma 7 on \ref{apbb} and $\tau = \arrow{\tau'_1}{\tau'_2}$\\
\>\la{tl}$\Theta'_1 \vdash \alphahat_1 \st \tau'_1 \dashv \Theta_1''$ \` Inversion of $\st\rightarrow$ on \ref{ast}\\
\>\la{tl2}$\Theta''_1 \vdash \tau'_2 \st \alphahat_2 \dashv \Theta_1$ \`\emph{ibid}\\
\>\la{hook1}$\Theta''_1 \hookrightarrow \Theta_1$ \` By lemma 32 on \ref{tl2}\\
\>\la{hook2}$\Theta''_1 \hookrightarrow \Theta_2$ \` By lemma 34 on \ref{hook1} and \ref{ctr2}\\
\>\la{thl1}$\Theta_2 \vdash \alphahat_1 \st \tau'_1 \dashv \Theta_2'$ \` By lemma 35 on \ref{tl} and \ref{hook2}\\
\>\la{th1pmt} $\Theta_2' \ctxmapto \Omega'$ \` By lemma 40 on \ref{thl1} and \ref{th2map}\\
\>\la{hook3}$\Theta_2 \hookrightarrow \Theta_2'$ \` By lemma 32 on \ref{thl1}\\
\>\la{hook4}$\Theta_1 \hookrightarrow \Theta_2'$ \` By lemma 34 on \ref{hook3}, \ref{ctr2}\\
\>\la{thl2}$\Theta_2' \vdash \tau'_2 \st \alphahat_2 \dashv \Theta_2''$ \` By lemma 32 on \ref{tl2} and \ref{taubnd3}\\
\>\la{th2pmt} $\Theta_2'' \ctxmapto \Omega'$ \` By lemma 41 on \ref{thl2} and \ref{th1pmt}\\
\>\la{lub1}$\Theta_2 \vdash \alphahat_1 \lub \tau'_1 = \alphahat_1 \dashv \Theta_2'$ \` Def. of $\lub$ on \ref{thl1}\\
\>\la{glb1}$\Theta_2' \vdash \alphahat_2 \glb \tau'_2 = \alphahat_2 \dashv \Theta_2''$ \` Def. of $\glb$ on \ref{thl2}\\
\>\la{alm1}$\Theta_2 \vdash \arrow{\tau_1'}{\tau_2'} \glb \arrow{\alphahat_1}{\alphahat_2} = \arrow{\alphahat_1}{\alphahat_2} \dashv \Theta_2''$ \` Defn. of $\glb$ on \ref{lub1} and \ref{glb1}\\
\>\la{fin1}$\Theta_2 \vdash \pair{\rho}{\tau} \glb \arrow{\alphahat_1}{\alphahat_2} = \pair{\rho}{\arrow{\alphahat_1}{\alphahat_2}} \dashv \Theta_3$ \` Choosing $\Theta_3 = \Theta_2''$\\
\>Case $\sigma_l = \pair{\rho}{\bot}$\\
\>\la{gls}$\Theta_2 \vdash \bot \glb \arrow{\alphahat_1}{\alphahat_2} = \arrow{\alphahat_1}{\alphahat_2} \dashv \Theta_2$\` By definition of $\glb$\\
\>\>$\Theta_2 \vdash \pair{\rho}{\bot} \glb \arrow{\alphahat_1}{\alphahat_2} = \pair{\rho}{\arrow{\alphahat_1}{\alphahat_2}} \dashv \Theta_3$ \` By definition of $\glb$ on \ref{gls} and choosing $\Theta_3=\Theta_2$\\
\>Case $\sigma_l = \pair{\rho}{\top}$\\
\>\>$\Gamma' \vdash \top \sigbndl \arrow{\tau_1}{\tau_2} \dashv \Omega$ \` By lemma 17 on \ref{taubnd}.\\
\>\>Contradiction\\
\>\la{th3mt}$\Theta_3 \ctxmapto \Omega'$ \` By \ref{gls} and \ref{th2pmt}\\
\la{2cont3}$\Theta_2 \hookrightarrow \Theta_3$ \` By lemma 33\\
\>$\sigma_t = \pair{\rho_t}{c_t}$\\
\la{lubk}$\Theta_3 \vdash \sigma_t \lub (\arrow{\alphahat_1}{\alphahat_2}) = \pair{\rho_t}{\arrow{\alphahat_1}{\alphahat_2}} \dashv \Theta_4$\\
\>Case \=$\sigma_t = \pair{\rho}{\tau}$\\
\>\la{bwave}$\Theta_1' \vdash \arrow{\alphahat_1}{\alphahat_2} \st \tau \dashv \Theta_2$ \` By lemma 33 on \ref{taubnd3}\\
\>\la{rep1}$\tau = \arrow{\tau_1'}{\tau_2'}$ \` Only $\st\rightarrow$ could have been used in \ref{bwave}, as $\tau$ monotype. Thus, $\tau$ is an arrow.\\
\>\la{rep2}$\Theta_1' \vdash \arrow{\alphahat_1}{\alphahat_2} \st \arrow{\tau_1'}{\tau_2'} \dashv \Theta_2$ \` By \ref{rep1}\\
\>\la{st1}$\Theta_1' \vdash \tau_1' \st \alphahat_1 \dashv \Theta_1''$\\
\>\la{st2}$\Theta_1'' \vdash \alphahat_2 \st \tau_2 \dashv \Theta_2$\\
\>\la{ct1}$\Theta_1' \hookrightarrow \Theta_1''$ \` Lemma 32 on \ref{st1}\\
\>\la{ct2}$\Theta_1'' \hookrightarrow \Theta_2$ \` Lemma 32 on \ref{st2}\\
\>\la{ct3}$\Theta_1' \hookrightarrow \Theta_3$ \` Lemma 34 on \ref{st1}, \ref{st2}, \ref{2cont3}\\
\>\la{bndext1}$\Theta_3 \vdash \tau_1' \st \alphahat_1 \dashv \Theta_3'$ \` By lemma 35 on \ref{ct3} and \ref{st1}\\
\>\la{th3pmt}$\Theta_3' \ctxmapto \Omega'$ \` By lemma 40 on \ref{th3mt} and \ref{bndext1}\\
\>\la{ct4}$\Theta_1'' \hookrightarrow \Theta_3'$ \` By lemma 34 on \ref{ct2}, \ref{2cont3}\\
\>\la{bndext2}$\Theta_3' \vdash \alphahat_2 \st \tau_2' \dashv \Theta_3''$ \` By lemma 35 on \ref{ct4} and \ref{st2}\\
\>\la{th3ppmt}$\Theta_3'' \ctxmapto \Omega'$ \` By lemma 41 on \ref{th3mt} and \ref{bndext2}\\
\>\la{glb2}$\Theta_3 \vdash \tau_1' \glb \alphahat_1 = \alphahat_1 \dashv \Theta_3'$ \` By definition of $\glb$ on \ref{bndext1}\\
\>\la{lub2}$\Theta_3'\vdash \alphahat_2 \lub \tau_2' = \alphahat_2 \dashv \Theta_3''$ \` By definition of $\lub$ of \ref{bndext2}\\
\>\la{lubfin} $\Theta_3 \vdash \arrow{\tau_1'}{\tau_2'} \lub \arrow{\alphahat_1}{\alphahat_2} = \arrow{\alphahat_1}{\alphahat_2} \dashv \Theta_4$ \`  By definition of $\lub$ on \ref{glb2} and \ref{lub2} and choose $\Theta_4 = \Theta_3''$\\
\>\la{3cont4}$\Theta_3 \hookrightarrow \Theta_4$ \` By lemmas 34 and 35 on \ref{bndext1} and \ref{bndext2}\\
\>\la{done1}$\Theta_3 \vdash \pair{\rho}{\tau} \lub (\arrow{\alphahat_1}{\alphahat_2}) = \pair{\rho}{\arrow{\alphahat_1}{\alphahat_2}} \dashv \Theta_4$\\
\>Case \=$\sigma_t = \pair{\rho}{\top}$\\
\>\>$\Theta_3 \vdash \pair{\rho}{\top} \glb \arrow{\alphahat_1}{\alphahat_2} = \pair{\rho}{\arrow{\alphahat_1}{\alphahat_2}} \dashv \Theta_3$ \` By defn. of $\glb$\\
\>Case \=$\sigma_t = \pair{\rho}{\bot}$\\
\>\la{ctra2}$\Theta_2 \vdash \arrow{\alphahat_1}{\alphahat_2} \sigbndr \pair{\rho}{\bot} \dashv \Theta_2$ \` By subst. on \ref{taubnd3}\\
\>\>$\Theta_2' \vdash \arrow{\alphahat_1}{\alphahat_2} \sigbndr \pair{\emptyset}{\bot} \dashv \Theta_2$ \`  By lemma 17 on \ref{ctra2}\\
\>\>Contradiction.\\
\>WTS: $\Theta_4[\bound{\pair{\rho_l}{\arrow{\alphahat_1}{\alphahat_2}}}{\alphahat}{\pair{\rho_t}{\arrow{\alphahat_1}{\alphahat_2}}}] \ctxmapto \Omega$\\
\>$\Theta_4[\bound{\pair{\rho_l}{\arrow{\alphahat_1}{\alphahat_2}}}{\alphahat}{\pair{\rho_t}{\arrow{\alphahat_1}{\alphahat_2}}}] = \Theta_4',\bound{\pair{\rho_l}{\arrow{\alphahat_1}{\alphahat_2}}}{\alphahat}{\pair{\rho_t}{\arrow{\alphahat_1}{\alphahat_2}}},\Theta_4''$ \` Def. of $\Theta_4$\\
\la{transcont}$\Gamma' \hookrightarrow \Theta_4$\` By lemma 34 on \ref{ctr1}, \ref{ctr2}, \ref{2cont3}, \ref{3cont4}\\
\la{transmap}$\Theta_4 \ctxmapto \Omega'$ \` By \ref{th3ppmt}, other cases are trivial\\
\la{break}$\Theta_4 = \Theta_4',\bound{\pair{\rho_l}{c_l}}{\alphahat}{\pair{\rho_t}{c_t}},\Theta_4''$ \` By construction of $\Theta_4$\\
\>$\Omega' = \Omega_u,\alphahat=\arrow{\tau_1}{\tau_2},\Omega_l$\\
\la{omm}$\Theta_4'' \ctxmapto \Omega_l$\\
\>WTS: $\Theta_4',\bound{\pair{\rho_l}{\arrow{\alphahat_1}{\alphahat_2}}}{\alphahat}{\pair{\rho_t}{\arrow{\alphahat_1}{\alphahat_2}}} \ctxmapto \Omega_u,\alphahat = \arrow{\tau_1}{\tau_2}$\\
\>WTS: $\Theta_4' \vdash \pair{\rho_l}{\arrow{\alphahat_1}{\alphahat_2}} \sigbndl \arrow{\tau_1}{\tau_2} \dashv \Theta$ and $\Theta \ctxmapto \Omega'$\\
\la{om1}$\Theta_4' \vdash \pair{\rho_l}{c_l} \sigbndl \arrow{\tau_1}{\tau_2} \dashv \_$ \` By lemma 10 on \ref{omm}\\
\la{breaklsig}$\Theta_4' \vdash \pair{\rho_l}{\bot} \sigbndl \arrow{\tau_1}{\tau_2} \dashv \Theta''$ \` By lemma 47 on \ref{om1}, for some $\Theta''$\\
\la{thppom}$\Theta'' \ctxmapto \Omega'$ \` \emph{ibid}\\
\>WTS $\Theta'' \vdash \arrow{\alphahat_1}{\alphahat_2} \st \arrow{\tau_1}{\tau_2} \dashv \Theta$\\
\la{ar1}$\Theta'' \vdash \tau_1 \st \alphahat_1 \dashv \Theta_{int}$ \`  Lem 50 on \ref{thppom}\\
\la{thiom}$\Theta_{int} \ctxmapto \Omega'$ \` \emph{ibid}\\
\la{ar2}$\Theta_{int} \vdash \alphahat_2 \st \tau_2 \dashv \Theta$ \` Lem 49 on \ref{thiom}\\
\la{thaom}$\Theta \ctxmapto \Omega'$ \` \emph{ibid}\\
\la{arlst}$\Theta'' \vdash \arrow{\alphahat_1}{\alphahat_2} \st \arrow{\tau_1}{\tau_2} \dashv \Theta$ \` By $\st\rightarrow$ on \ref{ar1} and \ref{ar2}\\
\la{bndl}$\Theta_4' \vdash \pair{\rho_l}{\arrow{\alphahat_1}{\alphahat_2}} \sigbndl \arrow{\tau_1}{\tau_2} \dashv \Theta$\` By lemma 12 on \ref{arlst} and \ref{breaklsig}\\
\>WTS: $\Theta_4' \vdash \arrow{\tau_1}{\tau_2} \sigbndr \pair{\rho_t}{\arrow{\alphahat_1}{\alphahat_2}} \dashv \Theta'$ and $\Theta' \ctxmapto \Omega'$\\
\la{om2}$\Theta_4' \vdash \arrow{\tau_1}{\tau_2} \sigbndr \pair{\rho_t}{c_t} \dashv \_$ \` By lemma 10 on \ref{omm}\\
\la{breakrsig}$\Theta_4' \vdash \arrow{\tau_1}{\tau_2} \sigbndl \pair{\rho_t}{\top} \dashv \Theta''$ \` By lemma 48 on \ref{om2}, for some $\Theta''$\\
\la{thppom2}$\Theta'' \ctxmapto \Omega'$ \` \emph{ibid}\\
\>WTS $\Theta'' \vdash \arrow{\tau_1}{\tau_2} \st \arrow{\alphahat_1}{\alphahat_2} \dashv \Theta'$\\
\la{ar3}$\Theta'' \vdash \alphahat_1 \st \tau_1 \dashv \Theta_{int}$ \`  Lem 49 on \ref{thppom2}\\
\la{thiom2}$\Theta_{int} \ctxmapto \Omega'$ \` \emph{ibid}\\
\la{ar4}$\Theta_{int} \vdash \tau_2 \st \alphahat_2 \dashv \Theta'$ \` Lem 40 on \ref{thiom2}\\
\la{thaom2}$\Theta' \ctxmapto \Omega'$ \` \emph{ibid}\\
\la{arrst}$\Theta'' \vdash \arrow{\tau_1}{\tau_2} \st \arrow{\alphahat_1}{\alphahat_2} \dashv \Theta'$ \` By $\st\rightarrow$ on \ref{ar1} and \ref{ar2}\\
\la{bndr} $\Theta_4' \vdash \arrow{\tau_1}{\tau_2} \sigbndr \pair{\rho_t}{\arrow{\alphahat_1}{\alphahat_2}} \dashv \Theta'$\` By lemma 12 on \ref{arrst} and \ref{breakrsig}\\
\la{comb}$\Theta_4',\bound{\pair{\rho_l}{\arrow{\alphahat_1}{\alphahat_2}}}{\alphahat}{\pair{\rho_t}{\arrow{\alphahat_1}{\alphahat_2}}},\Theta_4'' \ctxmapto \Omega_u,\alphahat = \arrow{\tau_1}{\tau_2},\Omega_l$ \` By lemma 11 on \ref{bndr}, \ref{bndl}, \ref{thaom}, \ref{thaom2}, \ref{omm}\\
\>$\Theta_{4,f} = \Theta_4',\bound{\pair{\rho_l}{\arrow{\alphahat_1}{\alphahat_2}}}{\alphahat}{\pair{\rho_t}{\arrow{\alphahat_1}{\alphahat_2}}},\Theta_4''$\\
\la{s1fhl} $[\Omega']\Theta_{4,f} \vdash \tau_1\leq [\Omega']A_1$ \` By \ref{comb} and \ref{declst1}\\
\la{pIH1} $[\Omega']\Theta_{4,f} \vdash [\Omega']\alphahat_1 \leq [\Omega']A_1$ \` As $\Omega'$ predicative and by \ref{s1fhl}\\
\> $\Theta_{4,f} \vdash \alphahat_1 \instl A_1 \dashv \Theta_5$ \` By IH on \ref{pIH1} and \ref{comb}\\
\la{cons} $\Theta_5 \ctxmapto \Omega'$ \` \emph{ibid}\\
\la{s2fhl} $[\Omega']\Theta_5 \vdash [\Omega']A_2 \leq \tau_2$ \` By \ref{comb} and \ref{declst2}\\
\la{pIH2} $[\Omega']\Theta_5 \vdash [\Omega']A_2 \leq [\Omega']\alphahat_2$ \` As $\Omega'$ predicative and by \ref{s2fhl}\\
\> $\Theta_5 \vdash A_2 \instr \alphahat_2 \dashv \Theta_6$ \` By IH on \ref{pIH2} and \ref{cons}\\
\> $\Theta_6 \ctxmapto \Omega'$ \` \emph{ibid}\\
\> Choose $\Delta = \Theta_6$\\
\> $\Gamma \vdash \alphahat \instl \arrow{A_1}{A_2} \dashv \Delta$ \` By InstLArrow on \ref{apbb}, \ref{taubnd3}, \ref{glb}, \ref{lubk}, \ref{pIH1}, and \ref{pIH2}\\
\>Again, remains to show the last component.\\
\end{tabbing}
\section{Instantiation Soundness}
\resla
Given $\Delta \mapsto \Omega$ and $\alphahat\not\in\text{FV}(A)$
\begin{tabbing}
$\Gamma \vdash A \st B \dashv \Delta \implies [\Omega]\Delta \vdash [\Omega]A \leq [\Omega]B$\\
$\Gamma \vdash \alphahat \instl A \dashv \Delta \implies [\Omega]\Delta \vdash [\Omega]\alphahat \leq [\Omega]A$\\
$\Gamma \vdash  A \instr \alphahat \dashv \Delta \implies [\Omega]\Delta \vdash [\Omega]A \leq [\Omega]\alphahat$\\
$\Gamma \vdash \pair{\{\betahat_1,\ldots,\betahat_n\}}{\tau} \sigbndl \tau' \dashv \Delta \implies$\\
\hspace{1em}\= $[\Omega]\Delta \vdash [\Omega]\betahat_1 \leq [\Omega]\tau$\\
\> $\ldots$\\
\> $[\Omega]\Delta \vdash [\Omega]\betahat_n \leq [\Omega]\tau$\\
\> $[\Omega]\Delta \vdash [\Omega]\tau \leq [\Omega]\tau'$\\
$\Gamma \vdash \tau \sigbndr \pair{\{\betahat_1,\ldots,\betahat_n\}}{\tau'} \dashv \Delta \implies$\\
\> $[\Omega]\Delta \vdash [\Omega]\alphahat \leq [\Omega]\betahat_1$\\
\> $\ldots$\\
\> $[\Omega]\Delta \vdash [\Omega]\alphahat \leq [\Omega]\betahat_n$\\
\> $[\Omega]\Delta \vdash [\Omega]\alphahat \leq [\Omega]\tau$\\
$\Gamma \vdash \pair{\{\betahat_1,\ldots,\betahat_n\}}{\tau} \glb \tau' = \pair{\{\betahat_1,\ldots,\betahat_n\}}{\tau''} \dashv \Delta \implies$\\
\> $[\Omega]\Delta \vdash [\Omega]\tau \leq [\Omega]\tau''$\\
\> $[\Omega]\Delta \vdash [\Omega]\tau' \leq [\Omega]\tau''$\\
$\Gamma \vdash \pair{\{\betahat_1,\ldots,\betahat_n\}}{\tau} \lub \tau' = \pair{\{\betahat_1,\ldots,\betahat_n\}}{\tau''} \dashv \Delta \implies$\\
\> $[\Omega]\Delta \vdash [\Omega]\tau'' \leq [\Omega]\tau$\\
\> $[\Omega]\Delta \vdash [\Omega]\tau'' \leq [\Omega]\tau'$\\
$\Gamma \vdash \tau \barwedge \tau' = \tau'' \dashv \Delta \implies$\\
\> $[\Omega]\Delta \vdash [\Omega]\tau \leq [\Omega]\tau''$\\
\> $[\Omega]\Delta \vdash [\Omega]\tau' \leq [\Omega]\tau''$\\
$\Gamma \vdash \tau \veebar \tau' = \tau'' \dashv \Delta \implies$\\
\> $[\Omega]\Delta \vdash [\Omega]\tau'' \leq [\Omega]\tau$\\
\> $[\Omega]\Delta \vdash [\Omega]\tau'' \leq [\Omega]\tau'$\\
\end{tabbing}

Proof.

Proceed by mutual rule induction.
\begin{tabbing}
\hspace{1em}\=\hspace{1em}\=\hspace{1em}\=\hspace{1em}\=\\
Instantiation:\\
\>Case InstLAbs\\
\>\>Given:\\
\>\>\la{des1}$\Gamma = \Gamma',\bound{\sigma_l}{\alphahat}{\sigma_u},\Gamma''$\\
\>\>\la{des2}$\Delta = \Delta',\bound{\sigma_l}{\alphahat}{\sigma_u},\Delta''$\\
\>\>\la{init1}$\Gamma' \vdash \sigma_l \sigbndl \tau \dashv \Theta$\\
\>\>\la{init2}$\Theta \vdash \sigma_u \lub \tau = \pair{\rho}{\tau'} \dashv \Delta'$\\
\>\>WTS:\\
\>\>\>$[\Omega]\Delta \vdash [\Omega]\alphahat \leq [\Omega]\tau$\\
\>\>$\Delta[\alphahat] \implies \Omega[\alphahat]$\\
\>\>$[\Omega]\alphahat = \tau_{sol}$\\
\>\la{solbnd}$\Delta\vdash \tau_{sol} \sigbndr \pair{\rho}{\tau'} \dashv\_$ \` As $\Delta \mapsto\Omega$\\
\>\>$[\Omega]\Delta \vdash [\Omega]\tau_{sol} \leq [\Omega]\tau'$ \` IH on \ref{solbnd}\\
\>\>$[\Omega]\Delta' \vdash [\Omega]\tau' \leq [\Omega]\tau$ \` IH on \ref{init2}\\
\>\>$[\Omega]\Delta \vdash [\Omega]\tau' \leq [\Omega]\tau$ \` As $\Delta' \hookrightarrow \Delta$ and by stability of instantiation.\\
\>\>$[\Omega]\Delta \vdash [\Omega]\tau_{sol} \leq [\Omega]\tau$\\
\>\>$[\Omega]\Delta \vdash [\Omega]\alphahat \leq [\Omega]\tau$\\
\>Case InstLReach\resla\\
\>\>Given:\\
\>\>\la{rdes1}$\Gamma = \Gamma',\bound{\pair{\{\rho_l\}}{\tau_l}}{\betahat}{\pair{\{\rho_u\}}{\tau_u}},\Gamma''$\\
\>\>\la{rdes2}$\Delta = \Delta',\bound{\pair{\{\rho_l,\alphahat\}}{\tau_l}}{\betahat}{\pair{\{\rho_u\}}{\tau_u}},\Delta''$\\
\>\>WTS:\\
\>\>\>$[\Omega]\Delta \vdash [\Omega]\alphahat \leq [\Omega]\betahat$\\
\>\>$\Delta[\betahat] \implies \Omega[\betahat]$\\
\>\>$[\Omega]\betahat = \tau_{sol}$\\
\>\la{solbnd2}$\Delta\vdash \pair{\{\rho_u,\alphahat\}}{\tau'} \sigbndl \tau_{sol} \dashv\_$ \` As $\Delta \mapsto\Omega$\\
\>\>$[\Omega]\Delta \vdash [\Omega]\alphahat \leq [\Omega]\tau_{sol}$ \` By IH on \ref{solbnd1}\\
\>\>$[\Omega]\Delta \vdash [\Omega]\alphahat \leq [\Omega]\betahat$ \` As $\Omega$ predicative\\
\>Case InstLArrow: (sketch)\\
\>\>$[\Omega]\alphahat=[\Omega]\alphahat_1\rightarrow[\Omega]\alphahat_2$ \` Derive from bounding + lub/glb relations\\
\>\>$[\Omega]\Delta \vdash [\Omega]A_1 \leq [\Omega]\alphahat_1$ \` IH on 2nd to last predicate\\
\>\>$[\Omega]\Delta \vdash [\Omega]\alphahat_2 \leq [\Omega]A_2$ \` IH on last predicate\\
\>\>$[\Omega]\Delta \vdash [\Omega]\alphahat_1 \rightarrow [\Omega]\alphahat_2 \leq [\Omega]A_1 \rightarrow [\Omega]A_2$\\
\>Case InstLAIIR and InstLAIIL\\
\>\>Identical to Dunfield's InstLAIIR.\\
\>Rest symmetric\\
Bounding \& Bound instantiation\\
\>Case BndLExt\\
\>\>$\forall \betahat \in \rho, [\Omega]\Gamma \vdash [\Omega]\betahat \leq [\Omega]\tau$ \` By IH.\\
\>\>$[\Omega]\Theta \vdash [\Omega]\alphahat \leq [\Omega]\tau$ \` By IH.\\
\>\>$\forall \betahat \in \rho, [\Delta]\Theta \vdash [\Delta]\betahat \leq [\Omega]\tau$ \` By bound contraction on 2.\\
\>\>$[\Omega]\Delta \vdash [\Omega]\alphahat \leq [\Omega]\tau$ \` By bound contraction on 2.\\
\>\>$\forall \betahat \in \{\alphahat,\rho\}, [\Omega]\Delta \vdash [\Omega]\betahat \leq [\Omega]\tau$\\
\>Case BndLBot\\
\>\>Trivial.\\
\>Case BndLType\\
\>\>Trivial by IH on precondition.\\
\>Case BndRExt\\
\>\>$\forall \betahat \in \rho, [\Omega]\Gamma \vdash [\Omega]\tau \leq [\Omega]\betahat$ \` By IH.\\
\>\>$[\Omega]\Theta \vdash [\Omega]\tau \leq [\Omega]\alphahat$ \` By IH.\\
\>\>$\forall \betahat \in \rho, [\Delta]\Theta \vdash [\Delta]\tau \leq [\Omega]\betahat$ \` By bound contraction on 2.\\
\>\>$[\Omega]\Delta \vdash [\Omega]\tau \leq [\Omega]\alphahat$ \` By bound contraction on 2.\\
\>\>$\forall \betahat \in \{\alphahat,\rho\}, [\Omega]\Delta \betahat [\Omega]\tau \leq [\Omega]\tau$\\
\>Case BndRBot\\
\>\>Trivial.\\
\>Case BndRType\\
\>\>Trivial by IH on precondition.\\
Glb/Lub\\
\> WTS: if $\Gamma \vdash \tau \veebar \tau' = \tau'' \dashv \Delta$, then $\forall A, \Delta \vdash A \st \tau \dashv \Delta'$ and $\Delta' \vdash A \st \tau' \dashv \Delta''$ then $[\Omega]\Delta \vdash [\Omega]A \leq [\Omega]\tau''$\\
\>Case\= $ \veebar\rightarrow$\\
\>\la{g1}$\Gamma \vdash \tau_1 \barwedge \tau_3 = \tau' \dashv \Theta$ \` Given.\\
\>\la{g2}$\Theta \vdash \tau_2 \veebar \tau_4 = \tau'' \dashv \Delta$ \` Given.\\
\>\la{g3}$\Gamma \vdash \tau_1 \rightarrow \tau_2 \veebar \tau_3 \rightarrow \tau_2 = \tau' \rightarrow \tau'' \dashv \Delta$ \` Given.\\
\>\>WTS: $\forall A, \Delta \vdash A \leq \tau_1 \rightarrow \tau_2 \dashv \Delta'$ and $\Delta' \vdash A \leq \tau_3 \rightarrow \tau_4 \dashv \Delta'' \implies [\Omega]\Delta \vdash [\Omega]A\leq [\Omega](\tau' \rightarrow \tau'')$\\
\>\> Suppose that there exists some $A$ s.t. $\Delta \vdash \tau_1 \rightarrow \tau_2 \st A \dashv \Delta'$ and $\Delta' \vdash \tau_3 \rightarrow \tau_4 \st A \vdash \Delta''$.\\
\>\la{st1} $[\Omega]\Delta \vdash [\Omega]A \leq [\Omega]\tau_1 \rightarrow [\Omega]\tau_2$. \` By soundness IH on given\\
\>\la{pst2} $[\Omega]\Delta' \vdash [\Omega]A \leq [\Omega]\tau_3 \rightarrow [\Omega] \tau_4$. \` By soundness IH on given\\
\>\la{st2} $[\Omega]\Delta \vdash [\Omega]A \leq [\Omega]\tau_3 \rightarrow [\Omega] \tau_4$. \` By stability of instantiation on \ref{pst2}\\
\>\la{inf} By inversion of $\leq\rightarrow$, for some $\tau_l, \tau_r$, $[\Omega]A = \tau_l \rightarrow \tau_r$.\\
\>\la{tll1}$[\Omega]\Delta \vdash [\Omega]\tau_1 \leq \tau_l$ \` By inversion of $\leq\rightarrow$ on \ref{inf} substituted into \ref{st1}\\
\>\la{tll2}$[\Omega]\Delta \vdash [\Omega]\tau_3 \leq \tau_l$ \` By inversion of $\leq\rightarrow$ on \ref{inf} substituted into \ref{st2}\\
\>\la{ext}$\Delta \vdash \tau_1 \barwedge \tau_3 = \tau''' \dashv \Delta$ and $[\Omega]\tau''' = [\Omega]\tau'$ \` By constraint propagation on $\Theta \hookrightarrow \Delta$\\ 
\>\la{r1}$[\Omega]\Delta \vdash [\Omega]\tau' \leq \tau_l$ \` By IH on \ref{tll1}, \ref{tll2}, and \ref{ext}\\
\>\la{tlr1}$[\Omega]\Delta \vdash \tau_r \leq [\Omega]\tau_2$ \` By inversion of $\leq\rightarrow$ on \ref{inf} substituted into \ref{st1}\\
\>\la{tlr2}$[\Omega]\Delta \vdash \tau_r \leq [\Omega]\tau_4$ \` By inversion of $\leq\rightarrow$ on \ref{inf} substituted into \ref{st2}\\
\>\la{r2}$[\Omega]\Delta \vdash \tau_r \leq [\Omega]\tau''$ \` By IH on \ref{tll1}, \ref{tll2}, and \ref{g2}\\
\>\>$[\Omega]\Delta \vdash \tau_l \rightarrow \tau_r \leq [\Omega](\tau' \rightarrow \tau'')$ \` $\leq\rightarrow$ on \ref{r1} and on \ref{r2}\\
\>\>$[\Omega]\Delta \vdash [\Omega]A \leq [\Omega](\tau' \rightarrow \tau'')$ \`  As $\Omega$ predicative.\\
\>Case $\veebar$L\\
\>Case $\veebar$R\\
\>Case $\veebar\exists $R \resla\\
\>\la{ge1}$\Gamma \vdash \betahat \instl A \dashv \Theta$ \` Given.\\
\>\la{ge2}$\Theta \vdash  \betahat \instr \alphahat \dashv \Delta$ \` Given.\\
\>\la{ge3}$\Gamma \vdash A \veebar \alphahat = \betahat \dashv \Delta$ \` Given.\\
\>\> Suppose that there exists some $B$ s.t. $\Delta \vdash B \st A \dashv \Delta'$ and $\Delta' \vdash B \st \alphahat \dashv \Delta''$.\\
\>\> Case \=on the rule used to conclude \ref{ge1}\\
\>\>\> Case \=InstLAbs or InstLReach\\
\>\>\>\>$A = \tau$ \` As InstLAbs concluded the proof.\\
\>\>\>\>Case \=on the structure of $\tau$\\
\>\>\>\>\> Case \=$\alphahat'$\\
\>\>\>\>\>\>$\Delta=\Delta',\pair{\emptyset}{\bot} \st \betahat \st \pair{\{\alphahat,\alphahat'\}}{\top}$ \` By application of InstLAbs\\
\>\>\>\>\>\>$\Delta \vdash B \instr \betahat \dashv \Delta'$ \` As $\Delta \vdash B \st \alphahat \dashv \Delta'$ and $\Delta \vdash B \st \alphahat' \dashv \Delta''$\\
\>\>\>\>\>\>$[\Omega]\Delta \vdash [\Omega]B \leq [\Omega] \betahat$ \` By soundness IH\\
\>\>\>\>\> Case $\tau$\\
\>\>\>\>\>\> $\Delta=\Delta',\pair{\emptyset}{\bot} \st \betahat \st \pair{\{\alphahat\}}{\tau}$ \` By application of InstLAbs\\
\>\>\>\>\>\>$\Delta \vdash B \instr \betahat \dashv \Delta'$ \` As $\Delta \vdash B \st \alphahat \dashv \Delta'$ and $\Delta \vdash B \st \tau \dashv \Delta''$\\
\>\>\>\>\>\>$[\Omega]\Delta \vdash [\Omega]B \leq [\Omega] \betahat$ \` By soundness IH\\
\>\>\> Case \=InstLArrow\\
\>\>\>\>$A = A_1 \rightarrow A_2$ \` As InstLArrow concluded the proof.\\
\>\>\>\>$\Delta=\Delta',\betahat_1,\betahat_2,\pair{\emptyset}{\bot} \st \betahat \st \pair{\{\alphahat\}}{\betahat_1 \rightarrow \betahat_2}$ \` By application of InstLArrow\\
\>\>\>\>$\Theta \dashv A_1 \instr \betahat_1 \dashv \Theta'$\\
\>\>\>\>$\Theta' \dashv \betahat_2 \instr A_2 \dashv \Delta$\\
\>\>\>\>$\Delta \vdash B \st A_1 \rightarrow A_2 \dashv \Delta'$\\
\>\>\>\>Case \=on the rule\\
\>\>\>\>\>Case \=$\st\rightarrow$\\
\>\>\>\>\>\>$B = B_1 \rightarrow B_2$\\
\>\>\>\>\>\>$\Delta \vdash A_1 \st B_1 \dashv \Theta$\\
\>\>\>\>\>\>$\Theta \vdash B_2 \st A_2 \dashv \Delta'$\\
Subtyping\\
\>More really simple inductions.\\
\end{tabbing}
The only interesting components of this proof are the instantiation judgments, the rest come from $\hookrightarrow$ and the IH directly. Note that the context size always decreases over the instantiation judgment, ensuring that the system is total.

This proof is quite simple and boring because the context extension precondition ensures that the output context is valid to a large degree, shifting the complexity to the completeness proof.

\paragraph{Bounding replacement lemmas}
\begin{tabbing}
WTS:\=\\
\>$\Gamma \vdash \tau \sigbndr \sigma_t \dashv \Delta$\\
\>$\Gamma \mapsto \Omega$\\
\>$[\Omega]\alphahat = \tau$\\
$\implies$\\
\>$\Gamma \vdash \alphahat \sigbndr \sigma_t \dashv \Delta'$\\
\>$\Delta' \mapsto \Omega$\\
\end{tabbing}


\paragraph{Unbounded existentials}
\begin{tabbing}
WTS:\=\\
\>$\Gamma[\bound{\pair{\emptyset}{\bot}}{\alphahat}{\pair{\emptyset}{\top}}]$\\
\>$\Gamma \vdash \alphahat \instl A_1 \dashv \Theta_1$\\
\>\ldots\\
\>$\Theta_n \vdash \alphahat \instl A_n \dashv \Theta$\\
\>$\Theta \vdash B \st A_1 \dashv \Delta_1$\\
\>\ldots\\
\>$\Delta_n \vdash B \st A_n \dashv \Delta$\\
$\implies$\\
\>$\Delta \vdash B \instr \alphahat \dashv \Delta'$\\
Proof.\\
Induct on $n$.\\
Case $n=0$: trivial.\\
Case \=$n=k$:\\
\>Proceed by rule induction on $\alphahat \instl A$.\\
\>Case \=InstLAbs or InstLReach\\
\>\>$A = \tau$ \` As InstLAbs concluded the proof.\\
\>\>Case \=on the structure of $\tau$\\
\>\>\> Case \=$\betahat'$\\
\>\>\>\>$\Delta=\Delta',\pair{\emptyset}{\bot} \st \alphahat \st \pair{\{\rho,\betahat'\}}{\tau}$ \` By application of InstLAbs\\
\>\>\>\>$\Delta \vdash B \instr \alphahat \dashv \Delta'$ \` As $\Delta \vdash B \st \alphahat \dashv \Delta'$ and $\Delta \vdash B \st \betahat' \dashv \Delta''$\\
\>\>\> Case $\tau$\\
\>\>\>\> $\Delta=\Delta',\pair{\emptyset}{\bot} \st \alphahat \st \pair{\{\alphahat\}}{\tau}$ \` By application of InstLAbs\\
\>\>\>\>$\Delta \vdash B \instr \alphahat \dashv \Delta'$ \` As $\Delta \vdash B \st \alphahat \dashv \Delta'$ and $\Delta \vdash B \st \tau \dashv \Delta''$\\
 Case \=InstLArrow\\
\>\>$A = A_1 \rightarrow A_2$ \` As InstLArrow concluded the proof.\\
\>\>$\Delta=\Delta',\alphahat_1,\alphahat_2,\pair{\emptyset}{\bot} \st \alphahat \st \pair{\{\alphahat\}}{\betahat_1 \rightarrow \betahat_2}$ \` By application of InstLArrow\\
\>\>$\Theta \dashv A_1 \instr \betahat_1 \dashv \Theta'$\\
\>\>$\Theta' \dashv \betahat_2 \instr A_2 \dashv \Delta$\\
\>\>$\Delta \vdash B \st A_1 \rightarrow A_2 \dashv \Delta'$\\
\>\>Case \=on the rule\\
\>\>\>Case \=$\st\rightarrow$\\
\>\>\>\>$B = B_1 \rightarrow B_2$\\
\>\>\>\>$\Delta \vdash A_1 \st B_1 \dashv \Theta$\\
\>\>\>\>$\Theta \vdash B_2 \st A_2 \dashv \Delta'$\\
\end{tabbing}
\end{document}